adapted HLPL/HLPL_plus to new name conventions

src/HLPL.v
@@ -14,104 +14,138 @@ Require Import OptionMonad.
 Local Open Scope option_monad_scope.
 Require Import SimulationUtils.
 
-Inductive HLPL_val :=
-| HLPL_bot : HLPL_val
-| HLPL_int : nat -> HLPL_val 
-| HLPL_loc : loan_id -> HLPL_val -> HLPL_val
-| HLPL_ptr : loan_id -> HLPL_val
-| HLPL_pair : HLPL_val -> HLPL_val -> HLPL_val
+(** * Definition of HLPL values and states. *)
+Inductive value :=
+| VBottom
+| VInt (n : nat) (* TODO: use Aeneas integer types? *)
+| VBool (b : bool)
+| VLoc (l : loan_id) (v : value)
+| VPtr (l : loan_id)
+| VTuple (t : list value)
 .
 
-Variant HLPL_nodes :=
-| HLPL_botC : HLPL_nodes
-| HLPL_intC : nat -> HLPL_nodes
-| HLPL_locC : loan_id -> HLPL_nodes
-| HLPL_ptrC : loan_id -> HLPL_nodes
-| HLPL_pairC : HLPL_nodes
+Fixpoint value_ind'
+  (P : value -> Type)
+  (fbot : P VBottom)
+  (fint : forall n, P (VInt n))
+  (fbool: forall b, P (VBool b))
+  (floc : ∀ l v, P v → P (VLoc l v))
+  (fptr : forall l, P (VPtr l))
+  (ftuple : ∀ vl : list value, ForallT P vl -> P (VTuple vl))
+  (v : value)
+  : P v :=
+  match v with
+  | VBottom => fbot
+  | VInt n => fint n
+  | VBool b => fbool b
+  | VLoc l v' => floc l v' (value_ind' P fbot fint fbool floc fptr ftuple v')
+  | VPtr l => fptr l
+  | VTuple vl =>
+      ftuple vl 
+      ((fix F vl :=
+        match vl as vl0 return ForallT P vl0 with
+        | [] => @ForallT_nil value P
+        | v' :: vl' =>
+            @ForallT_cons value P v' vl'
+              (value_ind' P fbot fint fbool floc fptr ftuple v')
+              (F vl')
+        end) vl)
+  end.
+
+Variant nodes :=
+| NBottom
+| NInt (n : nat)
+| NBool (b : bool)
+| NLoc (l : loan_id)
+| NPtr (l : loan_id)
+| NTuple (n : nat)
 .
 
-Instance EqDec_HLPL_nodes : EqDecision HLPL_nodes.
+Instance EqDec_HLPL_nodes : EqDecision nodes.
 Proof. unfold EqDecision, Decision. repeat decide equality. Qed.
 
 Definition HLPL_arity c := match c with
-| HLPL_botC => 0
-| HLPL_intC _ => 0
-| HLPL_locC _ => 1
-| HLPL_ptrC _ => 0
-| HLPL_pairC => 2
+| NBottom => 0
+| NInt _ => 0
+| NBool _ => 0
+| NLoc _ => 1
+| NPtr _ => 0
+| NTuple n => n
 end.
 
 Definition HLPL_get_node v := match v with
-| HLPL_bot => HLPL_botC
-| HLPL_int n => HLPL_intC n
-| HLPL_loc l _ => HLPL_locC l
-| HLPL_ptr l => HLPL_ptrC l
-| HLPL_pair _ _ => HLPL_pairC
+| VBottom => NBottom
+| VInt n => NInt n
+| VBool b => NBool b
+| VLoc l _ => NLoc l
+| VPtr l => NPtr l
+| VTuple t => NTuple (List.length t)
 end.
 
 Definition HLPL_children v := match v with
-| HLPL_bot => []
-| HLPL_int _ => []
-| HLPL_loc _ v => [v]
-| HLPL_ptr l => []
-| HLPL_pair fst snd => [fst ; snd]
+| VBottom => []
+| VInt _ => []
+| VBool _ => []
+| VLoc _ v => [v]
+| VPtr l => []
+| VTuple t => t
 end.
 
 Definition HLPL_fold c vs := match c, vs with
-| HLPL_intC n, [] => HLPL_int n
-| HLPL_locC l, [v] => HLPL_loc l v
-| HLPL_ptrC l, [] => HLPL_ptr l
-| HLPL_pairC, [fst; snd] => HLPL_pair fst snd
-| _, _ => HLPL_bot
+| NInt n, [] => VInt n
+| NBool b, [] => VBool b
+| NLoc l, [v] => VLoc l v
+| NPtr l, [] => VPtr l
+| NTuple n, t => VTuple t
+| _, _ => VBottom
 end.
 
 Fixpoint HLPL_weight node_weight v :=
   match v with
-  | HLPL_loc l v => node_weight (HLPL_locC l) + HLPL_weight node_weight v
-  | HLPL_pair fst snd =>
-      node_weight (HLPL_pairC) +
-        HLPL_weight node_weight fst + HLPL_weight node_weight snd
+  | VLoc l v => node_weight (NLoc l) + HLPL_weight node_weight v
+  | VTuple t => node_weight (HLPL_get_node (VTuple t)) +
+                 sum (map (HLPL_weight node_weight) t)
   | v => node_weight (HLPL_get_node v)
 end.
 
-Program Instance ValueHLPL : Value HLPL_val HLPL_nodes := {
+Program Instance ValueHLPL : Value value nodes := {
   arity := HLPL_arity;
   get_node := HLPL_get_node;
   children := HLPL_children;
   fold_value := HLPL_fold;
   vweight := HLPL_weight;
-  bot := HLPL_bot;
+  bot := VBottom;
 }.
 Next Obligation. destruct v; reflexivity. Qed.
 Next Obligation.
-  intros [] [] eq_node eq_children; inversion eq_node; inversion eq_children; reflexivity.
-Qed.
-Next Obligation.
-  intros [] ? H;
-  first [ rewrite length_zero_iff_nil in H; rewrite H
-        | destruct (length_1_is_singleton H) as [? ->]
-        | destruct (length_2_is_pair H) as [fst [snd ->] ] ];
-  reflexivity.
+  intros [] [] eq_node eq_children; inversion eq_node; inversion eq_children;
+    simpl in *; congruence. 
 Qed.
 Next Obligation.
  intros [] ? H;
   first [rewrite length_zero_iff_nil in H; rewrite H
-        | destruct (length_1_is_singleton H) as [? ->] 
-        | destruct (length_2_is_pair H) as [fst [snd ->] ] ];
+        | destruct (length_1_is_singleton H) as [? ->] | idtac ];
+   simpl in * ; congruence.
+Qed.
+Next Obligation.
+ intros [] ? H;
+  first [rewrite length_zero_iff_nil in H; rewrite H
+        | destruct (length_1_is_singleton H) as [? ->] | idtac ];
   reflexivity.
 Qed.
 Next Obligation. reflexivity. Qed.
-Next Obligation. intros ? []; unfold HLPL_children; cbn; lia. Qed.
+Next Obligation. intros ? []; unfold HLPL_children; cbn ; try lia.
+Qed.
 
-Record HLPL_state := {
-  vars : Pmap HLPL_val;
-  anons : Pmap HLPL_val;
+Record state := {
+  vars : Pmap value;
+  anons : Pmap value;
 }.
 
 Definition encode_var (x : var) := encode (A := var + anon) (inl x).
 Definition encode_anon (a : positive) := encode (A := var + anon) (inr a).
 
-Program Instance IsState : State HLPL_state HLPL_val (H := ValueHLPL) := {
+Program Instance IsState : State state value (H := ValueHLPL) := {
   extra := unit;
   get_map S := sum_maps (vars S) (anons S);
   get_extra _ := ();
@@ -129,21 +163,21 @@ Program Instance IsState : State HLPL_state HLPL_val (H := ValueHLPL) := {
     end;
   add_anon a v S := {| vars := vars S; anons := insert a v (anons S)|};
 }.
+Next Obligation. intros [? ?] [? ?]. cbn. intros (-> & ->)%sum_maps_eq _. reflexivity. Qed.
 Next Obligation. reflexivity. Qed.
 Next Obligation.
   intros ? ? i. cbn. destruct (decode' i) eqn:H.
   - rewrite decode'_is_Some in H.
     destruct s; cbn; rewrite <-H; symmetry;
       first [apply sum_maps_alter_inl | apply sum_maps_alter_inr].
-  - symmetry. apply map_alter_not_in_domain, sum_maps_lookup_None. assumption.
+  - symmetry. apply alter_id', sum_maps_lookup_None. assumption.
 Qed.
-Next Obligation. intros [? ?] [? ?]. cbn. intros (-> & ->)%sum_maps_eq _. reflexivity. Qed.
 (* What are the two following obligations? *)
 Next Obligation. discriminate. Qed.
 Next Obligation. discriminate. Qed.
+Next Obligation. reflexivity. Qed.
 Next Obligation. intros. cbn. symmetry. apply sum_maps_insert_inr. Qed.
 Next Obligation. reflexivity. Qed.
-Next Obligation. intros. unfold encode_anon. rewrite decode_encode. reflexivity. Qed.
 
 Lemma get_at_var S x : get_at_accessor S (encode_var x) = lookup x (vars S).
 Proof. unfold get_map, encode_var. cbn. apply sum_maps_lookup_l. Qed.
@@ -151,80 +185,39 @@ Proof. unfold get_map, encode_var. cbn. apply sum_maps_lookup_l. Qed.
 Declare Scope hlpl_scope.
 Delimit Scope hlpl_scope with hlpl.
 
-(* TODO: set every priority to 0? *)
-Reserved Notation "'loc' ( l , v )" (at level 0, l at next level, v at next level).
-Reserved Notation "'ptr' ( l )" (at level 0).
+(* Notation "'bot'" := VBottom: hlpl_plus_scope. *)
+Notation "'loc' ( l , v )" := (VLoc l v) : hlpl_scope.
+Notation "'ptr' ( l )" := (VPtr l) : hlpl_scope.
 
-Reserved Notation "'botC'" (at level 0).
-Reserved Notation "'locC' ( l , )" (at level 0, l at next level).
-Reserved Notation "'ptrC' ( l )" (at level 0).
-
-(* Notation "'bot'" := HLPL_bot: hlpl_scope. *)
-Notation "'loc' ( l , v )" := (HLPL_loc l v) : hlpl_scope.
-Notation "'ptr' ( l )" := (HLPL_ptr l) : hlpl_scope.
-
-Notation "'botC'" := HLPL_botC: hlpl_scope.
-Notation "'locC' ( l )" := (HLPL_locC l) : hlpl_scope.
-Notation "'ptrC' ( l )" := (HLPL_ptrC l) : hlpl_scope.
+Notation "'nbot'" := NBottom: hlpl_scope.
+Notation "'nloc' ( l )" := (NLoc l) : hlpl_scope.
+Notation "'nptr' ( l )" := (NPtr l) : hlpl_scope.
 
 (* Bind Scope hlpl_scope with HLPL_val. *)
 Open Scope hlpl_scope.
 
-Lemma sget_loc l v p : (loc(l, v)).[[ [0] ++  p]] = v.[[p]].
+Lemma sget_loc l v p : (loc (l, v)).[[ [0] ++  p]] = v.[[p]].
 Proof. reflexivity. Qed.
 Hint Rewrite sget_loc : spath.
 Lemma sget_loc' l v : (loc(l, v)).[[ [0] ]] = v.
 Proof. reflexivity. Qed.
 Hint Rewrite sget_loc' : spath.
 
-(* structural definition of not_value_contains *)
-Lemma valid_vpath_pair (vp : vpath) (v1 v2 : HLPL_val) : 
-  valid_vpath (HLPL_pair v1 v2) vp ->
-  (vp = []) \/ (exists vp', vp = 0 :: vp' ) \/ (exists vp', vp = 1 :: vp').
-Proof.
-  intros Hvp. destruct vp as [ _ | [ | [ | n ] ] vp' ].
-  - left; reflexivity.
-  - right ; left. exists vp'; reflexivity.
-  - right ; right. exists vp'; reflexivity.
-  - inversion Hvp ; subst. simpl in *. rewrite nth_error_nil in H2. easy.
-Qed.
-
-Lemma valid_vpath_loc (vp : vpath) (v : HLPL_val) : 
+Lemma valid_vpath_loc (vp : vpath) (v : value) : 
   forall l,
-  valid_vpath (HLPL_loc l v) vp ->
+  valid_vpath (loc (l, v)) vp ->
   (vp = []) \/ (exists vp', vp = 0 :: vp' ).
 Proof.
-  intros ? Hvp. destruct vp as [ _ | [ | n' ] vp' ].
+  intros ? Hvp. destruct vp as [ | [ | n' ] vp' ].
   - left; reflexivity.
   - right. exists vp'; reflexivity.
   - inversion Hvp ; subst. simpl in H2. rewrite nth_error_nil in H2. easy.
 Qed.
 
-Lemma not_value_contains_struct (v1 v2 : HLPL_val) (f : HLPL_nodes -> Prop) :
-  not_value_contains f (HLPL_pair v1 v2)
-  <-> not_value_contains f v1 /\ not_value_contains f v2 /\ ~ f HLPL_pairC.
-Proof.
-  split.
-  {
-    intros H. split ; [ idtac | split].
-    - intros p Hvp. apply (H (0 :: p)). eapply valid_cons ; auto.
-    - intros p Hvp. apply (H (1 :: p)). eapply valid_cons ; auto.
-    - apply (H []). apply valid_nil.
-  }
-  {
-    intros [H1 [ H2 Hp] ] p Hvp.
-    destruct (valid_vpath_pair p v1 v2 Hvp) as [ Hempty | [[vp' H] | [vp' H ] ] ] ;
-      subst ; simpl.
-    - assumption.
-    - apply H1. inversion Hvp; subst. injection H4 as Eq. congruence.
-    - apply H2. inversion Hvp; subst. injection H4 as Eq. congruence.
-  }
-Qed.
-
-Lemma not_value_contains_struct_loc (v : HLPL_val) (f : HLPL_nodes -> Prop) :
+Lemma not_value_contains_struct_loc (v : value) (f : nodes -> Prop) :
   forall l,
-  not_value_contains f (HLPL_loc l v)
-  <-> not_value_contains f v /\ ~ f (HLPL_locC l).
+  not_value_contains f (loc (l, v))
+  <-> not_value_contains f v /\ ~ f (nloc (l)).
 Proof.
   split.
   {
@@ -241,62 +234,57 @@ Proof.
 Qed.
 
 (* This property represents the application of a projection p (such as a pointer dereference or a
- * field access) on spath pi0, on a state S and given a permission perm.
- * If this projection is successful, then we have eval_proj S perm p pi0 pi1.
+ * field access) on spath pi0, on a state S.
+ * If this projection is successful, then we have eval_proj S p pi0 pi1.
  *)
-Variant eval_proj (S : HLPL_state) perm : proj -> spath -> spath -> Prop :=
+Variant eval_proj (S : state) : proj -> spath -> spath -> Prop :=
   (* Coresponds to R-Deref-Ptr-Loc and W-Deref-Ptr-Loc in the article. *)
-  | Eval_Deref_Ptr_Locs q q' l
-      (Hperm : perm <> Mov)
-      (get_q : get_node (S.[q]) = ptrC(l)) (get_q' : get_node (S.[q']) = locC(l)) :
-    eval_proj S perm Deref q q'
-  (* TODO: add fields *)
-  | Eval_Field_First q
-      (get_q : get_node (S.[q]) = HLPL_pairC) :
-    eval_proj S perm (Field First) q (q +++ [0])
-  | Eval_Field_Second q
-      (get_q : get_node (S.[q]) = HLPL_pairC) :
-    eval_proj S perm (Field Second) q (q +++ [1])
+  | E_Deref_Ptr_Locs q q' l
+      (get_q : get_node (S.[q]) = nptr(l)) (get_q' : get_node (S.[q']) = nloc(l)) :
+    eval_proj S Deref q q'
+  | E_Field q n k
+      (get_q : get_node (S.[q]) = NTuple n) (index: k < n) :
+    eval_proj S (Field k) q (q +++ [k])
 .
 
-Variant eval_loc (S : HLPL_state) perm : spath -> spath -> Prop :=
+Variant eval_loc (S : state) : spath -> spath -> Prop :=
   (* Coresponds to R-Loc and W-Loc in the article. *)
-  | Eval_Loc q l
-      (Hperm : perm <> Mov) (get_q : get_node (S.[q]) = locC(l)) :
-    eval_loc S perm q (q +++ [0])
+  | E_Loc q l
+      (get_q : get_node (S.[q]) = nloc(l)) :
+    eval_loc S q (q +++ [0])
 .
 
-(* Let pi0 be a spath. If by successfully applying the projections in P (with permission perm) we
-   obtain a spath pi1, then we have the proprety eval_path S perm P pi0 pi1. *)
-Inductive eval_path (S : HLPL_state) perm : path -> spath -> spath -> Prop :=
+(* Let pi0 be a spath. If by successfully applying the projections in P we
+   obtain a spath pi1, then we have the proprety eval_path S P pi0 pi1. *)
+Inductive eval_path (S : state) : path -> spath -> spath -> Prop :=
 (* Corresponds to R-Base and W-Base in the article. *)
-| Eval_nil pi : eval_path S perm [] pi pi
+| Eval_nil pi : eval_path S [] pi pi
 | Eval_cons proj P p q r
-    (Heval_proj : eval_proj S perm proj p q) (Heval_path : eval_path S perm P q r) :
-    eval_path S perm (proj :: P) p r
+    (Heval_proj : eval_proj S proj p q) (Heval_path : eval_path S P q r) :
+    eval_path S (proj :: P) p r
 | Eval_path_loc P p q r
-    (Heval_loc : eval_loc S perm  p q) (Heval_path_rec : eval_path S perm P q r) :
-    eval_path S perm P p r
+    (Heval_loc : eval_loc S p q) (Heval_path_rec : eval_path S P q r) :
+    eval_path S P p r
 .
 
-Definition eval_place S perm (p : place) pi :=
-  let pi_0 := (encode_var (fst p), []) in
-  valid_spath S pi_0 /\ eval_path S perm (snd p) (encode_var (fst p), []) pi.
+Definition eval_place S (p : place) pi :=
+  let pi_0 := (encode_var (fst (fst p)), []) in
+  valid_spath S pi_0 /\ eval_path S (snd (fst p)) (encode_var (fst (fst p)), []) pi.
 
-Notation "S  |-{p}  p =>^{ perm } pi" := (eval_place S perm p pi) (at level 50).
+Notation "S  |-{p}  p => pi" := (eval_place S p pi) (at level 50).
 
-Lemma eval_proj_valid S perm proj q r (H : eval_proj S perm proj q r) : valid_spath S r.
+Lemma eval_proj_valid S proj q r (H : eval_proj S proj q r) : valid_spath S r.
 Proof.
-  destruct H; validity.
+  destruct H ; validity.
 Qed.
 
-Lemma eval_loc_valid S perm q r (H : eval_loc S perm q r) : valid_spath S r.
+Lemma eval_loc_valid S q r (H : eval_loc S q r) : valid_spath S r.
 Proof.
-  destruct H; validity.
+  destruct H ; validity.
 Qed.
 
-Lemma eval_path_valid (s : HLPL_state) P perm q r
-  (valid_q : valid_spath s q) (eval_q_r : eval_path s perm P q r) :
+Lemma eval_path_valid (s : state) P q r
+  (valid_q : valid_spath s q) (eval_q_r : eval_path s P q r) :
   valid_spath s r.
 Proof.
   induction eval_q_r.
@@ -305,31 +293,31 @@ Proof.
   - apply IHeval_q_r. destruct Heval_loc. validity.
 Qed.
 
-Lemma eval_place_valid s p perm pi (H : eval_place s perm p pi) : valid_spath s pi.
+Lemma eval_place_valid s p pi (H : eval_place s p pi) : valid_spath s pi.
 Proof. destruct H as (? & ?). eapply eval_path_valid; eassumption. Qed.
 Hint Resolve eval_place_valid : spath.
 
-Variant is_loc : HLPL_nodes -> Prop :=
-| IsLoc_Loc l : is_loc (locC(l)).
+Variant is_loc : nodes -> Prop :=
+| IsLoc_Loc l : is_loc (nloc(l)).
 Definition not_contains_loc := not_value_contains is_loc.
 Hint Unfold not_contains_loc : spath.
 Hint Extern 0 (~is_loc _) => intro; easy : spath.
 
 Definition not_contains_bot v :=
-  (not_value_contains (fun c => c = botC) v).
+  (not_value_contains (fun c => c = nbot) v).
 Hint Unfold not_contains_bot : spath.
-Hint Extern 0 (_ <> botC) => discriminate : spath.
+Hint Extern 0 (_ <> nbot) => discriminate : spath.
 
 Definition get_loc_id c :=
   match c with
-  | locC(l) => Some l
-  | ptrC(l) => Some l
+  | nloc(l) => Some l
+  | nptr(l) => Some l
   | _ => None
   end.
 
 Notation is_fresh l S := (not_state_contains (fun c => get_loc_id c = Some l) S).
 
-Lemma is_fresh_loc_id_neq (S : HLPL_state) l0 l1 (p : spath) :
+Lemma is_fresh_loc_id_neq (S : state) l0 l1 (p : spath) :
   get_loc_id (get_node (S.[p])) = Some l0 -> is_fresh l1 S -> l0 <> l1.
 Proof.
   intros get_p Hfresh <-. eapply Hfresh; [ | exact get_p].
@@ -346,89 +334,161 @@ Hint Extern 0 (get_loc_id _ <> Some ?l) =>
       reflexivity
    end : spath.
 
-Inductive copy_val : HLPL_val -> HLPL_val -> Prop :=
-| Copy_val_int (n : nat) : copy_val (HLPL_int n) (HLPL_int n)
+(** ** Automation. *)
+(** A tactic to prove that a value or state does not contain some node (ex: loan, loc, bot).
+    This tactic tries to solve this by applying the relevant lemmas, and never fails. *)
+(* Note: Can we remove the automatic rewriting out of this tactic? *)
+(* TODO: precise the "workflow" of this tactic. *)
+Ltac not_contains0 :=
+  try assumption;
+  match goal with
+  | |- True => auto
+  | |- not_state_contains ?P (?S.[?p <- ?v]) =>
+      simple apply not_state_contains_sset;
+      not_contains0
+  | |- not_value_contains ?P (?S.[?q <- ?v].[?p]) =>
+      simple apply not_value_contains_sset_disj;
+        [auto with spath; fail | not_contains0]
+  | |- not_value_contains ?P (?S.[?q <- ?v].[?p]) =>
+      simple apply not_value_contains_sset;
+       [ not_contains0 | not_contains0 | validity0]
+  | H : not_state_contains ?P ?S |- not_value_contains ?P (?S.[?p]) =>
+      simple apply (not_state_contains_implies_not_value_contains_sget _ S p H);
+      validity0
+  | |- not_value_contains ?P (?v.[[?p <- ?w]]) =>
+      simple apply not_value_contains_vset; not_contains0
+  | |- not_value_contains ?P (?S.[?p]) => idtac
+
+  | |- not_value_contains ?P ?v =>
+      simple apply not_value_contains_zeroary; [reflexivity | ]
+  | |- not_value_contains ?P ?v =>
+      simple eapply not_value_contains_unary; [reflexivity | | not_contains0]
+  | |- not_value_contains ?P ?v =>
+      simple eapply not_value_contains_nary; [reflexivity | | not_contains0]
+  | |- _ => idtac
+  end.
+Ltac not_contains := not_contains0; eauto with spath.
+
+Inductive copy_val : value -> value -> Prop :=
+| Copy_val_int (n : nat) : copy_val (VInt n) (VInt n)
+| Copy_val_bool (b : bool) : copy_val (VBool b) (VBool b)
 | Copy_ptr l : copy_val (ptr(l)) (ptr(l))
 | Copy_loc l v w : copy_val v w -> copy_val (loc(l, v)) w
-| Copy_pair v1 v1' v2 v2' (H1 : copy_val v1 v1') (H2 : copy_val v2 v2') :
-  copy_val (HLPL_pair v1 v2) (HLPL_pair v1' v2').
+with copy_tuple_val : list value -> list value -> Prop :=
+| Copy_tuple_nil : copy_tuple_val [] []
+| Copy_tuple_cons vl1 vl2 v1 v2
+    (Hcopy : copy_val v1 v2)
+    (Hcopy_tuple : copy_tuple_val vl1 vl2) :
+  copy_tuple_val (v1 :: vl1) (v2 :: vl2).
 
 Reserved Notation "S  |-{op}  op  =>  r" (at level 60).
 
-Variant eval_operand : operand -> HLPL_state -> (HLPL_val * HLPL_state) -> Prop :=
-  | Eval_IntConst S n :
-    S |-{op} INT n => (HLPL_int n, S)
-  | Eval_copy S t (p : place) pi v
-      (Heval_place : eval_place S Imm p pi) (Hcopy_val : copy_val (S.[pi]) v) :
-    S |-{op} Copy t p => (v, S)
-  | Eval_move S t (p : place) pi :
-    eval_place S Mov p pi ->
+Inductive eval_operand : operand -> state -> (value * state) -> Prop :=
+  | E_IntConst S n : S |-{op} Const (IntConst n) => (VInt n, S)
+  | E_BoolConst S b : S |-{op} Const (BoolConst b) => (VBool b, S)
+  | E_Copy S (p : place) pi v
+      (Heval_place : eval_place S p pi) (Hcopy_val : copy_val (S.[pi]) v) :
+    S |-{op} Copy p => (v, S)
+  | E_Move S (p : place) pi :
+    eval_place S p pi ->
     not_contains_loc (S.[pi]) -> not_contains_bot (S.[pi]) ->
-    S |-{op} Move t p => (S.[pi], S.[pi <- bot])
-where "S |-{op} op => r" := (eval_operand op S r).
+    S |-{op} Move p => (S.[pi], S.[pi <- bot])
+  | E_Tuple S S' opl vl
+      (H : eval_tuple opl S (vl, S')) :
+    S |-{op} Tuple opl => (VTuple vl, S')
+where "S |-{op} op => r" := (eval_operand op S r)
+  with eval_tuple : list operand -> state -> (list value * state) -> Prop :=
+  | E_Tuple_Nil S : eval_tuple [] S ([], S)
+  | E_Tuple_Cons S S' S'' op opl v v'
+      (Hop : eval_operand op S (v, S'))
+      (Hrec : eval_tuple opl S' (v', S'')) :
+    eval_tuple (op :: opl) S (v :: v', S'')
+.
 
 Reserved Notation "S  |-{rv}  rv  =>  r" (at level 50).
 
-Variant eval_rvalue : rvalue -> HLPL_state -> (HLPL_val * HLPL_state) -> Prop :=
-  | Eval_just t op S vS' (Heval_op : S |-{op} op => vS') : S |-{rv} (Just t op) => vS'
-  (* For the moment, the only operation is the natural sum. *)
-  | Eval_bin_op S S' S'' t op_l op_r m n :
-      (S |-{op} op_l => (HLPL_int m, S')) ->
-      (S' |-{op} op_r => (HLPL_int n, S'')) ->
-      S |-{rv} (BinOp t op_l op_r) => ((HLPL_int (m + n)), S'')
-  | Eval_pointer_loc S t p pi l
-      (Heval_place : S |-{p} p =>^{Mut} pi)
-      (Hloc : get_node (S.[pi]) = locC(l)) : S |-{rv} &mut p : t => (ptr(l), S)
-  | Eval_pointer_no_loc S t p pi l
-      (* TODO *)
-      (Heval_place : S |-{p} p =>^{Mut} pi):
+Variant eval_binary_op : BinOp -> value -> value -> value -> Prop :=
+  | E_Add m n :
+      eval_binary_op BAdd (VInt m) (VInt n) (VInt (m + n))
+  | E_Le m n :
+      eval_binary_op BLe (VInt m) (VInt n) (VBool (m <=? n))
+.
+
+Variant eval_rvalue : rvalue -> state -> (value * state) -> Prop :=
+  | E_Use op S vS' (Heval_op : S |-{op} op => vS') : S |-{rv} (Use op) => vS'
+  | E_BinOp S S' S'' binop op_0 op_1 v0 v1 w
+      (eval_op_0 : S |-{op} op_0 => (v0, S'))
+      (eval_op_1 : S' |-{op} op_1 => (v1, S''))
+      (Hbinop : eval_binary_op binop v0 v1 w) :
+      S |-{rv} (BinaryOp binop op_0 op_1) => (w, S'')
+   | E_Pointer_Loc S p pi l
+      (Heval_place : S |-{p} p => pi)
+      (Hloc : get_node (S.[pi]) = nloc(l)) : S |-{rv} &mut p => (ptr(l), S)
+  | E_Pointer_Fresh S p pi l
+      (Heval_place : S |-{p} p => pi) :
       is_fresh l S ->
-      S |-{rv} (&mut p : t) => (ptr(l), (S.[pi <- loc(l, S.[pi])]))
-  | Eval_pair
-      S S' S'' v1 v2
-      fst_op t1 (Heval_first: eval_operand fst_op S (v1, S'))
-      snd_op t2 (Heval_first: eval_operand snd_op S' (v2, S'')) :
-    eval_rvalue (Pair (TPair t1 t2) fst_op snd_op) S ((HLPL_pair v1 v2), S'')
+      S |-{rv} (&mut p) => (VPtr(l), (S.[pi <- loc(l, S.[pi])]))
 where "S |-{rv} rv => r" := (eval_rvalue rv S r).
 (* TODO: add rule for pairs *)
 
-Lemma HLPL_Operand_NoLoc (S: HLPL_state) (op : operand) (vS : HLPL_val * HLPL_state) :
-  S |-{op} op => vS -> not_contains_loc vS.1 .
+Lemma copy_no_loc (v v' : value) :
+  copy_val v v' -> not_contains_loc v'
+with copy_tuple_no_loc (vl vl' : list value) :
+  copy_tuple_val vl vl' -> Forall not_contains_loc vl'.
 Proof.
-  intros [ | | ]; simpl ; try (unfold not_contains_loc ; not_contains).
-  induction Hcopy_val ; not_contains.
-  apply not_value_contains_struct ; repeat split ; auto.
-  intros H ; inversion H.
+  { intros copy. induction copy ; unfold not_contains_loc ; not_contains. }
+  { intros copy. induction copy ; constructor ; eauto. }
 Qed.
 
-Lemma HLPL_Rvalue_NoLoc (S: HLPL_state) (rv : rvalue) (vS : HLPL_val * HLPL_state) :
+Lemma eval_operand_no_loc (S : state) (op : operand) (vS' : value * state) :
+  S |-{op} op => vS' -> not_contains_loc vS'.1
+with  eval_tuple_no_loc (S : state) (opl : list operand) (vlS' : list value * state) :
+  eval_tuple opl S vlS' -> Forall (not_contains_loc) vlS'.1.
+Proof.
+  {
+    intros eval_op ; induction eval_op ;
+    try (unfold not_contains_loc ; not_contains).
+  + simpl. by apply copy_no_loc with (v := S.[ pi ]).
+  + simple eapply not_value_contains_nary ; [ easy |].
+    remember (vl, S') as vlS'. replace vl with (vlS'.1) by (subst ; reflexivity).
+    clear HeqvlS'. induction H.
+    - constructor.
+    - simpl in *. constructor ; [ | assumption].
+       replace v with ((v, S'0).1) by (simpl ; reflexivity).
+       apply eval_operand_no_loc with (S := S) (op := op) ; auto.
+  }
+  {
+    intros eval_t. induction eval_t ; [ constructor | ].
+    simpl. constructor ; [ | assumption ]. replace v with ((v, S').1) by reflexivity.
+    apply eval_operand_no_loc with (S := S) (op := op) ; auto.
+  }
+Qed.
+
+Lemma eval_rvalue_no_loc (S: state) (rv : rvalue) (vS : value * state) :
   S |-{rv} rv => vS -> not_contains_loc vS.1.
 Proof.
   intros Hrv ; induction Hrv ; try (unfold not_contains_loc ; not_contains).
-  - eapply HLPL_Operand_NoLoc, Heval_op.
-  - apply not_value_contains_struct.
-    apply HLPL_Operand_NoLoc in Heval_first, Heval_first0; simpl in *.
-    repeat split ; auto.
-    intros H ; inversion H.
+  - eapply eval_operand_no_loc, Heval_op.
+  - induction Hbinop ; simpl ; not_contains.
 Qed.
 
-Inductive reorg : HLPL_state -> HLPL_state -> Prop :=
+Inductive reorg : state -> state -> Prop :=
 | Reorg_end_ptr S (p : spath) l :
-    get_node (S.[p]) = ptrC(l) -> reorg S (S.[p <- bot])
+    get_node (S.[p]) = NPtr(l) -> reorg S (S.[p <- bot])
 | Reorg_end_loc S (p : spath) l :
-    get_node (S.[p]) = locC(l) -> not_state_contains (eq ptrC(l)) S ->
+    get_node (S.[p]) = NLoc(l) -> not_state_contains (eq (NPtr l)) S ->
     reorg S (S.[p <- S.[p +++ [0] ] ])
 .
 
 (* Automatically resolving the goals of the form `ptrC(l) <> _`, used to prove the condition
    `not_state_contains (eq ptrC(l)) S` of the rule Reorg_end_loc. *)
-Hint Extern 0 (ptrC( _ ) <> _) => discriminate : spath.
+Hint Extern 0 (NPtr( _ ) <> _) => discriminate : spath.
 
 (* This operation realizes the second half of an assignment p <- rv, once the rvalue v has been
  * evaluated to a pair (v, S). *)
-Variant store (p : place) : HLPL_val * HLPL_state -> HLPL_state -> Prop :=
+Variant store (p : place) : value * state -> state -> Prop :=
 | Store v S (sp : spath) (a : anon)
-  (eval_p : (S,, a |-> v) |-{p} p =>^{Mut} sp):
+  (eval_p : (S,, a |-> v) |-{p} p => sp):
   fresh_anon S a -> store p (v, S) (S.[sp <- v],, a |-> S.[sp])
 .
 
@@ -438,15 +498,15 @@ Variant store (p : place) : HLPL_val * HLPL_state -> HLPL_state -> Prop :=
 *)
 Reserved Notation "S  |-{stmt}  stmt  =>  r , S'" (at level 50).
 
-Inductive eval_stmt : statement -> statement_result -> HLPL_state -> HLPL_state -> Prop :=
-  | Eval_nop S : S |-{stmt} Nop => rUnit, S
-  | Eval_seq_unit S0 S1 S2 stmt_l stmt_r r (eval_stmt_l : S0 |-{stmt} stmt_l => rUnit, S1)
+Inductive eval_stmt : statement -> flow_token -> state -> state -> Prop :=
+  | E_Nop S : S |-{stmt} Nop => rUnit, S
+  | E_Seq_Unit S0 S1 S2 stmt_l stmt_r r (eval_stmt_l : S0 |-{stmt} stmt_l => rUnit, S1)
       (eval_stmt_r : S1 |-{stmt} stmt_r => r, S2) :  S0 |-{stmt} stmt_l;; stmt_r => r, S2
-  | Eval_seq_panic S0 S1 stmt_l stmt_r (eval_stmt_l : S0 |-{stmt} stmt_l => rPanic, S1) :
+  | E_Seq_Propagate S0 S1 stmt_l stmt_r (eval_stmt_l : S0 |-{stmt} stmt_l => rPanic, S1) :
       S0 |-{stmt} stmt_l;; stmt_r => rPanic, S1
-  | Eval_assign S vS' S'' p rv (eval_rv : S |-{rv} rv => vS') (Hstore : store p vS' S'') :
+  | E_Assign S vS' S'' p rv (eval_rv : S |-{rv} rv => vS') (Hstore : store p vS' S'') :
       S |-{stmt} ASSIGN p <- rv => rUnit, S''
-  | Eval_reorg S0 S1 S2 stmt r (Hreorg : reorg^* S0 S1) (Heval : S1 |-{stmt} stmt => r, S2) :
+  | E_Reorg S0 S1 S2 stmt r (Hreorg : reorg^* S0 S1) (Heval : S1 |-{stmt} stmt => r, S2) :
       S0 |-{stmt} stmt => r, S2
 where "S |-{stmt} stmt => r , S'" := (eval_stmt stmt r S S').
 
@@ -459,23 +519,26 @@ Proof.
   - rewrite H, nth_error_nil in G. inversion G.
 Qed.
 
-Fixpoint decide_not_value_contains (P : HLPL_nodes -> bool) v :=
+Fixpoint decide_not_value_contains (P : nodes -> bool) v :=
   negb (P (get_node v)) &&
     match v with
       loc(l, w) => decide_not_value_contains P w
-    | HLPL_pair v1 v2 =>
-        decide_not_value_contains P v1 &&
-          decide_not_value_contains P v2
+    | VTuple vl =>
+        forallb (decide_not_value_contains P) vl
     | _ => true end.
 
 Lemma decide_not_value_contains_correct H P v (H_implies_P : forall v, H v -> P v = true) :
   decide_not_value_contains P v = true -> not_value_contains H v.
 Proof.
-  intro decide_is_true. induction v.
+  intro decide_is_true. induction v using value_ind'.
   - intros p valid_p. apply valid_vpath_no_children in valid_p; [ | reflexivity].
     subst. cbn in *. intros G%H_implies_P. rewrite G in *. discriminate.
   - intros p valid_p. apply valid_vpath_no_children in valid_p; [ | reflexivity].
     subst. cbn in *. intros G%H_implies_P. rewrite G in *. discriminate.
+  - intros p valid_p. inversion valid_p; subst.
+    * cbn in *. intros G%H_implies_P.
+      apply andb_prop in decide_is_true as (? & _). rewrite G in H0. discriminate.
+    * rewrite nth_error_nil in H0. discriminate.
   - intros p valid_p. inversion valid_p; subst.
     + cbn in *.
       intros G%H_implies_P. rewrite G in decide_is_true. inversion decide_is_true.
@@ -486,25 +549,22 @@ Proof.
   - intros p valid_p. inversion valid_p; subst.
     + cbn in *. intros G%H_implies_P. rewrite G in decide_is_true. discriminate.
     + cbn in *. rewrite nth_error_nil in * |-. discriminate.
-  - intros p valid_p. inversion valid_p; subst.
-    + cbn in *. intros G%H_implies_P. rewrite G in decide_is_true. discriminate.
-    + cbn in *;
-      destruct (andb_prop _ _ decide_is_true);
-      destruct (andb_prop _ _ H3).
-      destruct i.
-      * cbn in *. apply IHv1. auto. congruence. 
-      * destruct i.
-        ** cbn in *. apply IHv2. auto. congruence.
-        ** cbn in *. rewrite nth_error_nil in H0. discriminate.
+  - intros p valid_p. inversion valid_p; subst ; cbn in *.
+    + intros G%H_implies_P. rewrite G in decide_is_true. discriminate.
+    + rewrite H1. apply (ForallT_nth _ vl i w) in H0 ; [ | assumption ].
+      apply H0 ; [ | assumption ].
+      apply andb_prop in decide_is_true as (_ & dit).
+      apply nth_error_In in H1.
+      apply forallb_forall with (x := w) in dit ; auto.
 Qed.
 
-Definition decide_is_bot v := match v with botC => true | _ => false end.
+Definition decide_is_bot v := match v with NBottom => true | _ => false end.
 
 Corollary decide_not_contains_bot v (H : decide_not_value_contains decide_is_bot v = true) :
   not_contains_bot v.
 Proof. eapply decide_not_value_contains_correct; try exact H. intros ? ->. reflexivity. Qed.
 
-Definition decide_not_state_contains (P : HLPL_nodes -> bool) (S : HLPL_state) :=
+Definition decide_not_state_contains (P : nodes -> bool) (S : state) :=
   map_fold (fun k v b => decide_not_value_contains P v && b) true (get_map S).
 
 Lemma decide_state_contains_correct H P S (H_implies_P : forall v, H v -> P v = true) :
@@ -520,10 +580,10 @@ Proof.
   - rewrite andb_false_l in G. discriminate.
 Qed.
 
-Definition decide_is_loc v := match v with locC(l) => true | _ => false end.
+Definition decide_is_loc v := match v with nloc(l) => true | _ => false end.
 Definition decide_is_loc_id l v :=
   match v with
-  | locC(l') | ptrC(l') => l =? l'
+  | nloc(l') | nptr(l') => Pos.eqb l l'
   | _ => false
   end.
 
@@ -532,7 +592,7 @@ Lemma decide_is_fresh S l (H : decide_not_state_contains (decide_is_loc_id l) S 
   is_fresh l S.
   Proof.
     eapply decide_state_contains_correct; try eassumption.
-    intros c G. destruct c; inversion G; apply Nat.eqb_refl.
+    intros c G. destruct c; inversion G; apply Pos.eqb_refl.
   Qed.
 
 
@@ -549,27 +609,27 @@ Notation a3 := 3%positive.
 Notation a4 := 4%positive.
 Notation a5 := 5%positive.
 Notation a6 := 6%positive.
-Notation l1 := 0%nat.
-Notation l2 := 1%nat.
+Notation l1 := 1%positive.
+Notation l2 := 2%positive.
 
 Definition prog :=
-  ASSIGN (x, nil) <- Just TInt (INT 3) ;;
-  ASSIGN (y, nil) <- &mut (1%positive, nil) : TRef.
+  ASSIGN (x, nil, TInt) <- Use (INT 3) ;;
+  ASSIGN (y, nil, TInt) <- &mut (1%positive, nil, TInt).
 
 Definition main : statement :=
-  ASSIGN (a, []) <- Just TInt (INT 1983) ;;
-  ASSIGN (b, []) <- Just TInt (INT 1986) ;;
-  ASSIGN (c, []) <- &mut (a, []) : TRef ;;
-  ASSIGN (d, []) <- &mut (c, [Deref]) : TRef ;;
-  ASSIGN (c, []) <- &mut (b, []) : TRef ;;
-  ASSIGN (d, [Deref]) <- Just TInt (INT 58) ;;
+  ASSIGN (a, [], TInt) <- Use (INT 1983) ;;
+  ASSIGN (b, [], TInt) <- Use (INT 1986) ;;
+  ASSIGN (c, [], TInt) <- &mut (a, [], TInt);;
+  ASSIGN (d, [], TInt) <- &mut (c, [Deref], TInt);;
+  ASSIGN (c, [], TInt) <- &mut (b, [], TInt);;
+  ASSIGN (d, [Deref], TInt) <- Use (INT 58) ;;
   Nop
 .
 
 Definition main_pair : statement :=
-  ASSIGN (a, []) <- Pair (TPair TInt TInt) (INT 667) (INT 1986) ;;
-  ASSIGN (b, []) <- Just TInt (Move TInt (a, [ Field (First)] )) ;;
-  ASSIGN (c, []) <- &mut (a, [Field (Second)]) : TRef ;;
+  ASSIGN (a, [], TTuple [TInt ; TInt]) <- Use (Tuple [ INT 667 ; INT 1986 ]) ;;
+  ASSIGN (b, [], TInt) <- Use (Move (a, [ Field (0)], TInt)) ;;
+  ASSIGN (c, [], TRef TInt) <- &mut (a, [Field (1)], TInt);;
   Nop
 .
 
@@ -591,11 +651,11 @@ Section SemTest.
     compute - [insert alter empty singleton];
     autorewrite with core.
 
-  Definition empty_state : HLPL_state :=
-    {| vars := {[ x := HLPL_int 0; y := HLPL_int 0 ]} ; anons := PEmpty |}.
-  Definition empty_state' : HLPL_state :=
+  Definition empty_state : state :=
+    {| vars := {[ x := VInt 0; y := VInt 0 ]} ; anons := PEmpty |}.
+  Definition empty_state' : state :=
     {|
-      vars := {[ a := HLPL_bot; b := HLPL_bot; c := HLPL_bot; d := HLPL_bot ]} ;
+      vars := {[ a := bot; b := bot; c := bot; d := bot ]} ;
       anons := PEmpty
     |}.
 
@@ -609,84 +669,71 @@ Section SemTest.
 
   Goal exists final_state, empty_state |-{stmt} prog => rUnit, final_state. 
     eexists.
-    eapply Eval_seq_unit.
+    eapply E_Seq_Unit.
     {
-      eapply Eval_assign.
+      eapply E_Assign.
       + repeat constructor.
       + apply Store with (a := a1).
         * eval_var; constructor.
         * reflexivity.
     }
     {
-      eapply Eval_assign.
-      + apply Eval_pointer_no_loc with (l := l1) (pi := (encode_var x, [])).
+      eapply E_Assign.
+      + simpl. eapply E_Pointer_Fresh with (l := l1).
         * eval_var; constructor.
-        * not_contains.
-          { apply decide_is_fresh. easy. }
-          unfold empty_state, encode_var, sget. simpl.
-          not_contains.
+        * apply decide_is_fresh. easy.
       + apply Store with (a := a2).
         * eval_var; constructor. 
-        * reflexivity. 
+        * reflexivity.
     }
   Qed.
 
   Goal exists final_state, empty_state' |-{stmt} main => rUnit, final_state.
     eexists.
-    eapply Eval_seq_unit.
+    eapply E_Seq_Unit.
     {
-      eapply Eval_assign.
+      eapply E_Assign.
       - repeat constructor.
-      - apply Store with (a := a1).
-        * eval_var; constructor.
-        * reflexivity.
+      - apply Store with (a := a1) ; [eval_var | ] ; constructor.
     }
     simpl_state.
-    eapply Eval_seq_unit.
+    eapply E_Seq_Unit.
     {
-      eapply Eval_assign.
+      eapply E_Assign.
       - repeat constructor.
-      - apply Store with (a := a2).
-        * eval_var; constructor.
-        * reflexivity.
+      - apply Store with (a := a2) ; [eval_var | ] ; constructor.
     }
     simpl_state.
-    eapply Eval_seq_unit.
+    eapply E_Seq_Unit.
     {
-      eapply Eval_assign.
-      - apply Eval_pointer_no_loc with (l := l1); repeat constructor.
+      eapply E_Assign.
+      - eapply E_Pointer_Fresh with (l := l1); repeat constructor.
         * eexists ; split; constructor; easy. (* TODO: why validity does not solve this goal? *)
         * apply decide_is_fresh. easy.
-      - apply Store with (a := a3).
-        * eval_var; constructor.
-        * reflexivity.
+      - apply Store with (a := a3) ; [eval_var | ] ; constructor.
     }
     simpl_state.
-    eapply Eval_seq_unit.
+    eapply E_Seq_Unit.
     {
-      eapply Eval_assign.
-      - apply Eval_pointer_loc with (pi := (encode_var 1, [])).
+      eapply E_Assign.
+      - apply E_Pointer_Loc with (pi := (encode_var 1, [])).
         * repeat econstructor; try easy.
         * reflexivity.
-      - apply Store with (a := a4).
-        * eval_var; constructor.
-        * reflexivity.
+      - apply Store with (a := a4) ; [eval_var | ] ; constructor.
     }
     simpl_state.
-    eapply Eval_seq_unit.
+    eapply E_Seq_Unit.
     {
-      eapply Eval_assign.
-      - apply Eval_pointer_no_loc with (l := l2); repeat constructor.
+      eapply E_Assign.
+      - apply E_Pointer_Fresh with (l := l2); repeat constructor.
         * eexists ; split; constructor; easy. (* TODO: why validity does not solve this goal? *)
         * apply decide_is_fresh. easy.
-      - apply Store with (a := a5).
-        * eval_var; constructor.
-        * reflexivity.
+      - apply Store with (a := a5) ; [eval_var | ] ; constructor.
     }
     simpl_state.
-    eapply Eval_seq_unit.
+    eapply E_Seq_Unit.
     {
-      eapply Eval_assign.
+      eapply E_Assign.
       - repeat constructor.
       - apply Store with (a := a6).
         * repeat constructor.
@@ -695,59 +742,50 @@ Section SemTest.
              repeat econstructor; easy.
         * reflexivity.
     }
-    apply Eval_nop.
+    apply E_Nop.
     Qed.
 
   Goal exists final_state, empty_state' |-{stmt} main_pair => rUnit, final_state.
     eexists.
-    eapply Eval_seq_unit.
+    eapply E_Seq_Unit.
     {
-      eapply Eval_assign.
+      eapply E_Assign.
       - repeat econstructor.
-      - apply Store with (a := a1); repeat constructor.
-        validity.
-        * simpl. eexists; split; constructor.
-        * reflexivity.
+      - apply Store with (a := a1) ; [eval_var | ] ; constructor.
     }
     simpl_state.
-    eapply Eval_seq_unit.
+    eapply E_Seq_Unit.
     {
-      eapply Eval_assign.
+      eapply E_Assign.
       - repeat econstructor. 
         * apply decide_not_value_contains_correct with (P := decide_is_loc).
           ** intros. inversion H; subst; reflexivity.
           ** reflexivity.
         * apply decide_not_contains_bot; reflexivity.
-      - apply Store with (a := a2); repeat constructor.
-        validity.
-        * simpl. eexists; split; constructor.
-        * reflexivity.
+      - apply Store with (a := a2) ; [eval_var | ] ; constructor.
     }
     simpl_state.
-    eapply Eval_seq_unit.
+    eapply E_Seq_Unit.
     {
-      eapply Eval_assign.
-      - apply Eval_pointer_no_loc with (l := l1).
+      eapply E_Assign.
+      - apply E_Pointer_Fresh with (l := l1).
         * repeat econstructor.
         * apply decide_is_fresh; reflexivity.
-      - apply Store with (a := a3); repeat constructor.
-        validity.
-        * simpl. eexists; split; constructor.
-        * reflexivity.
+      - apply Store with (a := a3) ; [eval_var | ] ; constructor.
     }
-    apply Eval_nop.
+    apply E_Nop.
     Qed.
 End SemTest.
 
 
-Record HLPL_well_formed (S : HLPL_state) : Prop := {
-  at_most_one_loc l : at_most_one_node (locC(l)) S;
+Record HLPL_well_formed (S : state) : Prop := {
+  at_most_one_loc l : at_most_one_node (nloc(l)) S;
 }.
 
 Notation scount c S := (sweight (indicator c) S).
 
-Record HLPL_well_formed_alt (S : HLPL_state) l : Prop := {
-  at_most_one_loc_alt : scount (locC(l)) S <= 1;
+Record HLPL_well_formed_alt (S : state) l : Prop := {
+  at_most_one_loc_alt : scount (nloc(l)) S <= 1;
 }.
 
 Lemma well_formedness_equiv S : HLPL_well_formed S <-> forall l, HLPL_well_formed_alt S l.
@@ -760,19 +798,19 @@ Proof.
 Qed.
 
 Lemma vweight_loc weight l v :
-  vweight weight (loc(l, v)) = weight (locC(l)) + vweight weight v.
+  vweight weight (loc(l, v)) = weight (nloc(l)) + vweight weight v.
 Proof. reflexivity. Qed.
 Hint Rewrite vweight_loc : weight.
 
-Lemma vweight_ptr weight l : vweight weight (ptr(l)) = weight (ptrC(l)).
+Lemma vweight_ptr weight l : vweight weight (ptr(l)) = weight (nptr(l)).
 Proof. reflexivity. Qed.
 Hint Rewrite vweight_ptr : weight.
 
 Lemma vweight_int weight n :
-  vweight weight (HLPL_int n) = weight (HLPL_intC n).
+  vweight weight (VInt n) = weight (NInt n).
 Proof. reflexivity. Qed.
 Hint Rewrite vweight_int : weight.
 
-Lemma vweight_bot weight : vweight weight bot = weight (botC).
+Lemma vweight_bot weight : vweight weight bot = weight (nbot).
 Proof. reflexivity. Qed.
 Hint Rewrite vweight_bot : weight.
